import Relation.Binary.PropositionalEquality as Eq
open Eq using (_≡_; refl; cong; sym)
open Eq.≡-Reasoning using (begin_; _≡⟨⟩_; step-≡; _∎)
open import Data.Nat using (ℕ; zero; suc; _+_; _*_; _∸_)

+-assoc′ : ∀ (m n p : ℕ) → (m + n) + p ≡ m + (n + p)
+-assoc′ zero    n p                          =  refl
+-assoc′ (suc m) n p  rewrite +-assoc′ m n p  =  refl

+-identity′ : ∀ (n : ℕ) → n + zero ≡ n
+-identity′ zero = refl
+-identity′ (suc n) rewrite +-identity′ n = refl

+-suc′ : ∀ (m n : ℕ) → m + suc n ≡ suc (m + n)
+-suc′ zero n = refl
+-suc′ (suc m) n rewrite +-suc′ m n = refl

+-comm′ : ∀ (m n : ℕ) → m + n ≡ n + m
+-comm′ m zero rewrite +-identity′ m = refl
+-comm′ m (suc n) rewrite +-suc′ m n | +-comm′ m n = refl
