import Relation.Binary.PropositionalEquality as Eq
open Eq using (_≡_; refl; cong; sym)
open Eq.≡-Reasoning using (begin_; _≡⟨⟩_; step-≡; _∎)
open import Data.Nat using (ℕ; zero; suc; _+_; _*_; _∸_)

-- ∧ ∨
-- P ∧ true = P
-- P ∨ false = P
-- P ∧ (Q ∧ R) = (P ∧ Q) ∧ R
-- P ∨ (Q ∨ R) = (P ∨ Q) ∨ R
-- P ∧ (Q ∨ R) = (P ∧ Q) ∨ (P ∧ R)
-- ⟹
-- P ⟹ (Q ⟹ R) = (P ⟹ Q) ⟹ R
-- P ⟹ Q ≢ Q ⟹ P

+-assoc : ∀ (m n p : ℕ) → (m + n) + p ≡ m + (n + p)
+-assoc zero n p =
  begin
    (zero + n) + p
  ≡⟨⟩
    n + p
  ≡⟨⟩
    zero + (n + p)
  ∎
+-assoc (suc m) n p =
  begin
    (suc m + n) + p
  ≡⟨⟩
    suc (m + n) + p
  ≡⟨⟩
    suc ((m + n) + p)
  ≡⟨ cong suc (+-assoc m n p) ⟩
    suc (m + (n + p))
  ≡⟨⟩
    suc m + (n + p)
  ∎


+-assoc-2 : ∀ (n p : ℕ) → (2 + n) + p ≡ 2 + (n + p)
+-assoc-2 n p =
  begin
    (2 + n) + p
  ≡⟨⟩
    suc (1 + n) + p
  ≡⟨⟩
    suc ((1 + n) + p)
  ≡⟨ cong suc (+-assoc-1 n p) ⟩
    suc (1 + (n + p))
  ≡⟨⟩
    2 + (n + p)
  ∎
  where
  +-assoc-1 : ∀ (n p : ℕ) → (1 + n) + p ≡ 1 + (n + p)
  +-assoc-1 n p =
    begin
      (1 + n) + p
    ≡⟨⟩
      suc (0 + n) + p
    ≡⟨⟩
      suc ((0 + n) + p)
    ≡⟨ cong suc (+-assoc-0 n p) ⟩
      suc (0 + (n + p))
    ≡⟨⟩
      1 + (n + p)
    ∎
    where
    +-assoc-0 : ∀ (n p : ℕ) → (0 + n) + p ≡ 0 + (n + p)
    +-assoc-0 n p =
      begin
        (0 + n) + p
      ≡⟨⟩
        n + p
      ≡⟨⟩
        0 + (n + p)
      ∎

+-rearrange : ∀ (m n p q : ℕ) → (m + n) + (p + q) ≡ m + (n + p) + q
+-rearrange m n p q =
  begin
    (m + n) + (p + q)
  ≡⟨ +-assoc m n (p + q) ⟩
    m + (n + (p + q))
  ≡⟨ cong (m +_) (sym (+-assoc n p q)) ⟩
    m + ((n + p) + q)
  ≡⟨ sym (+-assoc m (n + p) q) ⟩
    (m + (n + p)) + q
  ≡⟨⟩
    m + (n + p) + q
  ∎